libcrux-ml-kem/proofs/fstar/extraction/Libcrux_ml_kem.Vector.Portable.Arithmetic.fst
@@ -3,7 +3,32 @@ module Libcrux_ml_kem.Vector.Portable.Arithmetic
 open Core
 open FStar.Mul
 
-let get_n_least_significant_bits (n: u8) (value: u32) = value &. ((1ul <<! n <: u32) -! 1ul <: u32)
+#push-options "--z3rlimit 150 --split_queries always"
+
+let get_n_least_significant_bits (n: u8) (value: u32) =
+  let res:u32 = value &. ((1ul <<! n <: u32) -! 1ul <: u32) in
+  let _:Prims.unit =
+    calc ( == ) {
+      v res;
+      ( == ) { () }
+      v (logand value ((1ul <<! n) -! 1ul));
+      ( == ) { mk_int_equiv_lemma #u32_inttype 1 }
+      v (logand value (((mk_int 1) <<! n) -! (mk_int 1)));
+      ( == ) { () }
+      v (logand value (mk_int ((1 * pow2 (v n)) % pow2 32) -! (mk_int 1)));
+      ( == ) { (Math.Lemmas.small_mod (pow2 (v n)) (pow2 32);
+        Math.Lemmas.pow2_lt_compat 32 (v n)) }
+      v (logand value ((mk_int (pow2 (v n))) -! (mk_int 1)));
+      ( == ) { (Math.Lemmas.pow2_lt_compat 32 (v n);
+        logand_mask_lemma value (v n)) }
+      v value % (pow2 (v n));
+    }
+  in
+  res
+
+#pop-options
+
+#push-options "--z3rlimit 150"
 
 let barrett_reduce_element (value: i16) =
   let t:i32 =
@@ -13,8 +38,34 @@ let barrett_reduce_element (value: i16) =
       i32) +!
     (Libcrux_ml_kem.Vector.Traits.v_BARRETT_R >>! 1l <: i32)
   in
+  let _:Prims.unit =
+    assert_norm (v v_BARRETT_MULTIPLIER == (pow2 27 + 3329) / (2 * 3329));
+    assert (v t = v value * v v_BARRETT_MULTIPLIER + pow2 25)
+  in
+  let _:Prims.unit = assert (v t / pow2 26 < 9) in
+  let _:Prims.unit = assert (v t / pow2 26 > - 9) in
   let quotient:i16 = cast (t >>! Libcrux_ml_kem.Vector.Traits.v_BARRETT_SHIFT <: i32) <: i16 in
-  value -! (quotient *! Libcrux_ml_kem.Vector.Traits.v_FIELD_MODULUS <: i16)
+  let _:Prims.unit = assert (v quotient = v t / pow2 26) in
+  let _:Prims.unit = assert (Spec.Utils.is_i16b 9 quotient) in
+  let result:i16 = value -! (quotient *! Libcrux_ml_kem.Vector.Traits.v_FIELD_MODULUS <: i16) in
+  let _:Prims.unit =
+    calc ( == ) {
+      v result % 3329;
+      ( == ) { () }
+      (v value - (v quotient * 3329)) % 3329;
+      ( == ) { Math.Lemmas.lemma_mod_sub_distr (v value) (v quotient * 3329) 3329 }
+      (v value - (v quotient * 3329) % 3329) % 3329;
+      ( == ) { Math.Lemmas.cancel_mul_mod (v quotient) 3329 }
+      (v value - 0) % 3329;
+      ( == ) { () }
+      (v value) % 3329;
+    }
+  in
+  result
+
+#pop-options
+
+#push-options "--z3rlimit 300 --split_queries always"
 
 let montgomery_reduce_element (value: i32) =
   let _:i32 = v_MONTGOMERY_R in
@@ -22,16 +73,93 @@ let montgomery_reduce_element (value: i32) =
     (cast (cast (value <: i32) <: i16) <: i32) *!
     (cast (Libcrux_ml_kem.Vector.Traits.v_INVERSE_OF_MODULUS_MOD_MONTGOMERY_R <: u32) <: i32)
   in
+  let _:Prims.unit =
+    assert (v (cast (cast (k <: i32) <: i16) <: i32) == v k @% pow2 16);
+    assert (v (cast (cast (k <: i32) <: i16) <: i32) < pow2 15);
+    assert (v (cast (cast (k <: i32) <: i16) <: i32) >= - pow2 15);
+    assert (v (cast (Libcrux_ml_kem.Vector.Traits.v_FIELD_MODULUS <: i16) <: i32) == 3329)
+  in
   let k_times_modulus:i32 =
     (cast (cast (k <: i32) <: i16) <: i32) *!
     (cast (Libcrux_ml_kem.Vector.Traits.v_FIELD_MODULUS <: i16) <: i32)
   in
+  let _:Prims.unit =
+    Spec.Utils.lemma_mul_i16b (pow2 15)
+      (3329)
+      (cast (k <: i32) <: i16)
+      Libcrux_ml_kem.Vector.Traits.v_FIELD_MODULUS;
+    assert (Spec.Utils.is_i32b (pow2 15 * 3329) k_times_modulus)
+  in
   let c:i16 = cast (k_times_modulus >>! v_MONTGOMERY_SHIFT <: i32) <: i16 in
+  let _:Prims.unit =
+    assert (v k_times_modulus < pow2 31);
+    assert (v k_times_modulus / pow2 16 < pow2 15);
+    assert (v c == (v k_times_modulus / pow2 16) @% pow2 16);
+    assert (v c == v k_times_modulus / pow2 16);
+    assert (Spec.Utils.is_i16b 1665 c)
+  in
   let value_high:i16 = cast (value >>! v_MONTGOMERY_SHIFT <: i32) <: i16 in
-  value_high -! c
+  let _:Prims.unit =
+    assert (v value < pow2 31);
+    assert (v value / pow2 16 < pow2 15);
+    assert (v value_high == (v value / pow2 16) @% pow2 16);
+    assert (v value_high == (v value / pow2 16));
+    assert (Spec.Utils.is_i16b 3328 value_high)
+  in
+  let res:i16 = value_high -! c in
+  let _:Prims.unit = assert (Spec.Utils.is_i16b (3328 + 1665) res) in
+  let _:Prims.unit =
+    calc ( == ) {
+      v k_times_modulus % pow2 16;
+      ( == ) { () }
+      ((v k @% pow2 16) * 3329) % pow2 16;
+      ( == ) { () }
+      ((((v value @% pow2 16) * 62209) @% pow2 16) * 3329) % pow2 16;
+      ( == ) { Math.Lemmas.lemma_mod_sub ((((v value @% pow2 16) * 62209) % pow2 16) * 3329)
+        (pow2 16)
+        3329 }
+      ((((v value @% pow2 16) * 62209) % pow2 16) * 3329) % pow2 16;
+      ( == ) { Math.Lemmas.lemma_mod_mul_distr_l ((v value @% pow2 16) * 62209) 3329 (pow2 16) }
+      ((((v value @% pow2 16) * 62209) * 3329) % pow2 16);
+      ( == ) { Math.Lemmas.lemma_mod_mul_distr_r (v value @% pow2 16) (62209 * 3329) (pow2 16) }
+      ((v value @% pow2 16) % pow2 16);
+      ( == ) { () }
+      (v value) % pow2 16;
+    };
+    Math.Lemmas.modulo_add (pow2 16) (- (v k_times_modulus)) (v value) (v k_times_modulus);
+    assert ((v value - v k_times_modulus) % pow2 16 == 0)
+  in
+  let _:Prims.unit =
+    calc ( == ) {
+      v res % 3329;
+      ( == ) { () }
+      (v value / pow2 16 - v k_times_modulus / pow2 16) % 3329;
+      ( == ) { Math.Lemmas.lemma_div_exact (v value - v k_times_modulus) (pow2 16) }
+      ((v value - v k_times_modulus) / pow2 16) % 3329;
+      ( == ) { () }
+      (((v value - v k_times_modulus) / pow2 16) * ((pow2 16 * 62209) % 3329)) % 3329;
+      ( == ) { Math.Lemmas.lemma_mod_mul_distr_r ((v value - v k_times_modulus) / pow2 16)
+        (pow2 16 * 62209)
+        3329 }
+      (((v value - v k_times_modulus) / pow2 16) * pow2 16 * 62209) % 3329;
+      ( == ) { Math.Lemmas.lemma_div_exact (v value - v k_times_modulus) (pow2 16) }
+      ((v value - v k_times_modulus) * 62209) % 3329;
+      ( == ) { () }
+      ((v value * 62209) - ((v k @% pow2 16) * 3329 * 62209)) % 3329;
+      ( == ) { Math.Lemmas.lemma_mod_sub (v value * 62209) 3329 ((v k @% pow2 16) * 62209) }
+      (v value * 62209) % 3329;
+    }
+  in
+  let result:i16 = res in
+  let _:Prims.unit = admit () (* Panic freedom *) in
+  result
+
+#pop-options
 
 let montgomery_multiply_fe_by_fer (fe fer: i16) =
-  montgomery_reduce_element ((cast (fe <: i16) <: i32) *! (cast (fer <: i16) <: i32) <: i32)
+  let _:Prims.unit = Spec.Utils.lemma_mul_i16b (pow2 16) (3328) fe fer in
+  let product:i32 = (cast (fe <: i16) <: i32) *! (cast (fer <: i16) <: i32) in
+  montgomery_reduce_element product
 
 #push-options "--admit_smt_queries true"
 
