libcrux-ml-kem/proofs/fstar/extraction/Libcrux_ml_kem.Vector.Traits.fsti
@@ -126,38 +126,50 @@ class t_Operations (v_Self: Type0) = {
         (f_decompress_ciphertext_coefficient_pre v_COEFFICIENT_BITS x0)
         (fun result -> f_decompress_ciphertext_coefficient_post v_COEFFICIENT_BITS x0 result);
   f_ntt_layer_1_step_pre:a: v_Self -> zeta0: i16 -> zeta1: i16 -> zeta2: i16 -> zeta3: i16
-    -> pred: Type0{true ==> pred};
+    -> pred:
+      Type0
+        { Spec.Utils.is_i16b 1664 zeta0 /\ Spec.Utils.is_i16b 1664 zeta1 /\
+          Spec.Utils.is_i16b 1664 zeta2 /\ Spec.Utils.is_i16b 1664 zeta3 ==>
+          pred };
   f_ntt_layer_1_step_post:v_Self -> i16 -> i16 -> i16 -> i16 -> v_Self -> Type0;
   f_ntt_layer_1_step:x0: v_Self -> x1: i16 -> x2: i16 -> x3: i16 -> x4: i16
     -> Prims.Pure v_Self
         (f_ntt_layer_1_step_pre x0 x1 x2 x3 x4)
         (fun result -> f_ntt_layer_1_step_post x0 x1 x2 x3 x4 result);
-  f_ntt_layer_2_step_pre:a: v_Self -> zeta0: i16 -> zeta1: i16 -> pred: Type0{true ==> pred};
+  f_ntt_layer_2_step_pre:a: v_Self -> zeta0: i16 -> zeta1: i16
+    -> pred: Type0{Spec.Utils.is_i16b 1664 zeta0 /\ Spec.Utils.is_i16b 1664 zeta1 ==> pred};
   f_ntt_layer_2_step_post:v_Self -> i16 -> i16 -> v_Self -> Type0;
   f_ntt_layer_2_step:x0: v_Self -> x1: i16 -> x2: i16
     -> Prims.Pure v_Self
         (f_ntt_layer_2_step_pre x0 x1 x2)
         (fun result -> f_ntt_layer_2_step_post x0 x1 x2 result);
-  f_ntt_layer_3_step_pre:a: v_Self -> zeta: i16 -> pred: Type0{true ==> pred};
+  f_ntt_layer_3_step_pre:a: v_Self -> zeta: i16
+    -> pred: Type0{Spec.Utils.is_i16b 1664 zeta ==> pred};
   f_ntt_layer_3_step_post:v_Self -> i16 -> v_Self -> Type0;
   f_ntt_layer_3_step:x0: v_Self -> x1: i16
     -> Prims.Pure v_Self
         (f_ntt_layer_3_step_pre x0 x1)
         (fun result -> f_ntt_layer_3_step_post x0 x1 result);
   f_inv_ntt_layer_1_step_pre:a: v_Self -> zeta0: i16 -> zeta1: i16 -> zeta2: i16 -> zeta3: i16
-    -> pred: Type0{true ==> pred};
+    -> pred:
+      Type0
+        { Spec.Utils.is_i16b 1664 zeta0 /\ Spec.Utils.is_i16b 1664 zeta1 /\
+          Spec.Utils.is_i16b 1664 zeta2 /\ Spec.Utils.is_i16b 1664 zeta3 ==>
+          pred };
   f_inv_ntt_layer_1_step_post:v_Self -> i16 -> i16 -> i16 -> i16 -> v_Self -> Type0;
   f_inv_ntt_layer_1_step:x0: v_Self -> x1: i16 -> x2: i16 -> x3: i16 -> x4: i16
     -> Prims.Pure v_Self
         (f_inv_ntt_layer_1_step_pre x0 x1 x2 x3 x4)
         (fun result -> f_inv_ntt_layer_1_step_post x0 x1 x2 x3 x4 result);
-  f_inv_ntt_layer_2_step_pre:a: v_Self -> zeta0: i16 -> zeta1: i16 -> pred: Type0{true ==> pred};
+  f_inv_ntt_layer_2_step_pre:a: v_Self -> zeta0: i16 -> zeta1: i16
+    -> pred: Type0{Spec.Utils.is_i16b 1664 zeta0 /\ Spec.Utils.is_i16b 1664 zeta1 ==> pred};
   f_inv_ntt_layer_2_step_post:v_Self -> i16 -> i16 -> v_Self -> Type0;
   f_inv_ntt_layer_2_step:x0: v_Self -> x1: i16 -> x2: i16
     -> Prims.Pure v_Self
         (f_inv_ntt_layer_2_step_pre x0 x1 x2)
         (fun result -> f_inv_ntt_layer_2_step_post x0 x1 x2 result);
-  f_inv_ntt_layer_3_step_pre:a: v_Self -> zeta: i16 -> pred: Type0{true ==> pred};
+  f_inv_ntt_layer_3_step_pre:a: v_Self -> zeta: i16
+    -> pred: Type0{Spec.Utils.is_i16b 1664 zeta ==> pred};
   f_inv_ntt_layer_3_step_post:v_Self -> i16 -> v_Self -> Type0;
   f_inv_ntt_layer_3_step:x0: v_Self -> x1: i16
     -> Prims.Pure v_Self
@@ -170,7 +182,11 @@ class t_Operations (v_Self: Type0) = {
       zeta1: i16 ->
       zeta2: i16 ->
       zeta3: i16
-    -> pred: Type0{true ==> pred};
+    -> pred:
+      Type0
+        { Spec.Utils.is_i16b 1664 zeta0 /\ Spec.Utils.is_i16b 1664 zeta1 /\
+          Spec.Utils.is_i16b 1664 zeta2 /\ Spec.Utils.is_i16b 1664 zeta3 ==>
+          pred };
   f_ntt_multiply_post:v_Self -> v_Self -> i16 -> i16 -> i16 -> i16 -> v_Self -> Type0;
   f_ntt_multiply:x0: v_Self -> x1: v_Self -> x2: i16 -> x3: i16 -> x4: i16 -> x5: i16
     -> Prims.Pure v_Self
